Optimizations/Canonicalizations/AddPhase.thy
@@ -29,13 +29,13 @@ proof -
   from xv yv have "intval_add x y = IntVal b (take_bit b (xv+yv))" (is "_ = IntVal b ?val")
     using assms
     using intval_add.simps(1) by presburger
-  then have "constantAsStamp (intval_add x y) = (IntegerStamp b (int_signed_value b ?val) (int_signed_value b ?val))" (is "_ = ?stamp")
+  then have csdef: "constantAsStamp (intval_add x y) = (IntegerStamp b (signed_take_bit (b-1) ?val) (signed_take_bit (b-1) ?val) (and (take_bit b (xv + yv)) (mask b)) (and (take_bit b (xv+yv)) (mask b)))" (is "_ = ?stamp")
     using constantAsStamp.simps(1) by presburger
   then have "valid_stamp ?stamp"
     by (metis assms(3) constantAsStamp.simps(1) validStampIntConst valid_stamp.simps(1) valid_value.simps(1) wf_value_def yv)
   then show ?thesis 
     using valid_value.simps(1)
-    by (simp add: \<open>intval_add x y = IntVal b (take_bit b (xv + yv))\<close> wf_value_def)
+    using \<open>intval_add x y = IntVal b (take_bit b (xv + yv))\<close> validDefIntConst wf_value_def by auto
 qed
 
 optimization AddFold:
@@ -44,13 +44,14 @@ optimization AddFold:
   using wf_value_intval_add by blast
 
 thm AddFold_code
+thm AddFold
 
 lemma binadd_commute:
   assumes "bin_eval BinAdd x y \<noteq> UndefVal"
   shows "bin_eval BinAdd x y = bin_eval BinAdd y x"
   by (simp add: intval_add_sym)
 
-optimization AddShiftConstantRight[nogen]:
+optimization AddShiftConstantRight:
   when "cond[x instanceof ConstantNode]"
   when "cond[!(y instanceof ConstantNode)]"
   "(x + y) \<longmapsto> (y + x)"
